alias_simple: implementation and proofs

examples/alias_simple.dfy
@@ -1,5 +1,6 @@
 include "../lib/NativeTypes.s.dfy"
 include "../lib/MutableMap.i.dfy"
+include "../lib/Option.s.dfy"
 
 module GraphSpec {
   import opened NativeTypes
@@ -79,16 +80,17 @@ module GraphSpec {
 }
 
 module FunctionalGraph /* refines GraphSpec */ {
+  import opened NativeTypes
   import S = GraphSpec
 
   type Reference = S.Reference
 
   datatype Constants = Constants
 
-  datatype GraphValue = GraphValue(adjList: set<Reference>, rc: int)
+  datatype GraphValue = GraphValue(adjList: set<Reference>, rc: uint64)
   datatype Variables = Variables(
       graph: map<Reference, GraphValue>,
-      invRc: map<int, set<Reference>>,
+      invRc: map<uint64, set<Reference>>,
       nextRef: Reference)
 
   function Ik(k: Constants): S.Constants
@@ -105,12 +107,16 @@ module FunctionalGraph /* refines GraphSpec */ {
   {
     && S.Inv(Ik(k), I(k, s))
 
+    && (forall ref | ref in s.graph :: ref !in s.graph[ref].adjList)
+
     && (forall r | r in s.graph :: (
       && var c := s.graph[r].rc;
       && c in s.invRc
       && r in s.invRc[c]))
     && (forall c | c in s.invRc :: forall r | r in s.invRc[c] :: r in s.graph)
     && (forall c | c in s.invRc :: forall r | r in s.invRc[c] :: s.graph[r].rc == c)
+
+    && (forall ref | ref in s.graph :: (exists r | r in s.graph :: ref in s.graph[r].adjList) ==> s.graph[ref].rc > 0)
   }
 
   function Init(k: Constants): (s': Variables)
@@ -132,6 +138,7 @@ module FunctionalGraph /* refines GraphSpec */ {
     AllocResult(
       s
         .(graph := s.graph[s.nextRef := GraphValue({}, 0)])
+        .(invRc := s.invRc[0 := (if 0 in s.invRc then s.invRc[0] else {}) + {s.nextRef}])
         .(nextRef := s.nextRef + 1),
       s.nextRef)
   }
@@ -152,6 +159,7 @@ module FunctionalGraph /* refines GraphSpec */ {
       && r in s'.invRc[c]));
     assume forall c | c in s'.invRc :: forall r | r in s'.invRc[c] :: r in s'.graph;
     assume forall c | c in s'.invRc :: forall r | r in s'.invRc[c] :: s'.graph[r].rc == c;
+    assume forall ref | ref in s'.graph :: (exists r | r in s'.graph :: ref in s'.graph[r].adjList) ==> s'.graph[ref].rc > 0;
     assert Inv(k, s');
     assume ref !in s.graph;
     assert S.Alloc(Ik(k), I(k, s), I(k, s'), Alloc(k, s).ref);
@@ -197,6 +205,8 @@ module FunctionalGraph /* refines GraphSpec */ {
     && parent in s.graph
     && ref in s.graph
     && ref !in s.graph[parent].adjList
+    && parent != ref
+    && s.graph[ref].rc as nat < 0x1_0000_0000_0000_0000 - 1
   }
 
   function Attach(k: Constants, s: Variables, parent: Reference, ref: Reference): (s': Variables)
@@ -273,6 +283,7 @@ module FunctionalGraph /* refines GraphSpec */ {
       && r in s'.invRc[c]));
     assume forall c | c in s'.invRc :: forall r | r in s'.invRc[c] :: r in s'.graph;
     assume forall c | c in s'.invRc :: forall r | r in s'.invRc[c] :: s'.graph[r].rc == c;
+    assume forall ref | ref in s'.graph :: (exists r | r in s'.graph :: ref in s'.graph[r].adjList) ==> s'.graph[ref].rc > 0;
     assert Inv(k, s');
     assume I(k, s').graph == I(k, s).graph[parent := (I(k, s).graph[parent] - {ref})];
     assert S.Detach(Ik(k), I(k, s), I(k, s'), parent, ref);
@@ -349,6 +360,8 @@ module FunctionalGraph /* refines GraphSpec */ {
 }
 
 module ImperativeGraph /* refines FunctionalGraph */ {
+  import opened NativeTypes
+  import opened Options
   import MutableMap
   import F = FunctionalGraph
 
@@ -356,14 +369,19 @@ module ImperativeGraph /* refines FunctionalGraph */ {
   type GraphValue = F.GraphValue
   type Reference = F.Reference
 
-  class State {
+  lemma {:axiom} CountBoundedByMemory<V(==)>(h: HashMap<V>)
+  requires h.Inv()
+  ensures h.Count as nat < 0x10000000000000000 / 8
+
+  class Impl {
     var graph: HashMap<GraphValue>;
     var invRc: HashMap<set<Reference>>;
-    var nextRef: int;
+    var nextRef: uint64;
 
     ghost var Repr: set<object>;
 
     constructor()
+    ensures WFImpl(this)
     {
       graph := new MutableMap.ResizingHashMap<GraphValue>(1024);
       invRc := new MutableMap.ResizingHashMap<set<Reference>>(256);
@@ -371,7 +389,183 @@ module ImperativeGraph /* refines FunctionalGraph */ {
 
       new;
 
-      Repr := graph.Repr + invRc.Repr;
+      Repr := {this} + graph.Repr + invRc.Repr;
     }
+  }
+
+  predicate WFImpl(impl: Impl)
+  ensures WFImpl(impl) ==> {impl, impl.graph, impl.invRc} <= impl.Repr
+  reads impl, impl.Repr
+  {
+    && {impl, impl.graph, impl.invRc} <= impl.Repr
+    && impl.Repr == {impl} + impl.graph.Repr + impl.invRc.Repr
+
+    && impl.graph.Inv()
+    && impl.invRc.Inv()
+  }
+
+  function Ik(impl: Impl): F.Constants
+  {
+    F.Constants()
+  }
+
+  function I(impl: Impl): F.Variables
+  requires WFImpl(impl)
+  reads impl.Repr
+  {
+    F.Variables(
+      MutableMap.ResizingHashMap.I(impl.graph),
+      MutableMap.ResizingHashMap.I(impl.invRc),
+      impl.nextRef)
+  }
+
+  predicate Inv(impl: Impl)
+  requires WFImpl(impl)
+  reads impl.Repr
+  {
+    && F.Inv(Ik(impl), I(impl))
+  }
+
+  function method UnwrapOr<T>(opt: Option<T>, otherwise: T): T
+  {
+    match opt {
+      case Some(x) => x
+      case None => otherwise
+    }
+  }
+
+  method Alloc(impl: Impl) returns (ref: Reference)
+  requires WFImpl(impl)
+  requires F.AllocRequires(Ik(impl), I(impl))
+  requires Inv(impl)
+  ensures WFImpl(impl)
+  ensures Inv(impl)
+  ensures F.Next(old(Ik(impl)), old(I(impl)), I(impl))
+  modifies impl.Repr
+  {
+    ref := impl.nextRef;
+    impl.nextRef := impl.nextRef + 1;
+    CountBoundedByMemory(impl.graph);
+    var _ := impl.graph.Insert(ref, F.GraphValue({}, 0));
+    var invRc0opt := impl.invRc.Get(0);
+    var invRc0 := UnwrapOr(invRc0opt, {}) + {ref};
+    CountBoundedByMemory(impl.invRc);
+    var _ := impl.invRc.Insert(0, invRc0);
+
+    impl.Repr := {impl} + impl.graph.Repr + impl.invRc.Repr;
+
+    ghost var ghostRef := F.RefinesAlloc(old(Ik(impl)), old(I(impl)), I(impl));
+    assert ref == ghostRef;
+    assert F.NextStep(old(Ik(impl)), old(I(impl)), I(impl), F.AllocStep());
+  }
+
+  method Dealloc(impl: Impl, ref: Reference)
+  requires WFImpl(impl)
+  requires F.DeallocRequires(Ik(impl), I(impl), ref)
+  requires Inv(impl)
+  ensures WFImpl(impl)
+  ensures Inv(impl)
+  ensures F.Next(old(Ik(impl)), old(I(impl)), I(impl))
+  modifies impl.Repr
+  {
+    var _ := impl.graph.Remove(ref);
+    var invRc0opt := impl.invRc.Get(0);
+    assert invRc0opt.Some?;
+    var invRc0 := invRc0opt.value - {ref};
+    CountBoundedByMemory(impl.invRc);
+    var _ := impl.invRc.Insert(0, invRc0);
+
+    impl.Repr := {impl} + impl.graph.Repr + impl.invRc.Repr;
+
+    F.RefinesDealloc(old(Ik(impl)), old(I(impl)), I(impl), ref);
+    assert F.NextStep(old(Ik(impl)), old(I(impl)), I(impl), F.DeallocStep(ref));
+  }
+
+  method Attach(impl: Impl, parent: Reference, ref: Reference)
+  requires WFImpl(impl)
+  requires F.AttachRequires(Ik(impl), I(impl), parent, ref)
+  requires Inv(impl)
+  ensures WFImpl(impl)
+  ensures Inv(impl)
+  ensures F.Next(old(Ik(impl)), old(I(impl)), I(impl))
+  modifies impl.Repr
+  {
+    assert impl.graph.Repr !! impl.invRc.Repr;
+    assert WFImpl(impl);
+
+    var parentEl := impl.graph.Get(parent);
+    assert parentEl.Some?;
+    var newParentEl := parentEl.value.(adjList := (parentEl.value.adjList + {ref}));
+    CountBoundedByMemory(impl.graph);
+    var _ := impl.graph.Insert(parent, newParentEl);
+    impl.Repr := {impl} + impl.graph.Repr + impl.invRc.Repr;
+
+    var refEl := impl.graph.Get(ref);
+    assert refEl.Some?;
+    var newRefEl := refEl.value.(rc := refEl.value.rc + 1);
+    CountBoundedByMemory(impl.graph);
+    var _ := impl.graph.Insert(ref, newRefEl);
+    impl.Repr := {impl} + impl.graph.Repr + impl.invRc.Repr;
+
+    var invRcAopt := impl.invRc.Get(refEl.value.rc);
+    assert invRcAopt.Some?;
+    var invRcA := invRcAopt.value - {ref};
+    CountBoundedByMemory(impl.invRc);
+    var _ := impl.invRc.Insert(refEl.value.rc, invRcA);
+    impl.Repr := {impl} + impl.graph.Repr + impl.invRc.Repr;
+
+    var invRcBopt := impl.invRc.Get(refEl.value.rc + 1);
+    var invRcB := UnwrapOr(invRcBopt, {}) + {ref};
+    CountBoundedByMemory(impl.invRc);
+    var _ := impl.invRc.Insert(refEl.value.rc + 1, invRcB);
+    impl.Repr := {impl} + impl.graph.Repr + impl.invRc.Repr;
+
+    assert I(impl) == F.Attach(old(Ik(impl)), old(I(impl)), parent, ref);
+    F.RefinesAttach(old(Ik(impl)), old(I(impl)), I(impl), parent, ref);
+    assert F.NextStep(old(Ik(impl)), old(I(impl)), I(impl), F.AttachStep(parent, ref));
+  }
+
+  method Detach(impl: Impl, parent: Reference, ref: Reference)
+  requires WFImpl(impl)
+  requires F.DetachRequires(Ik(impl), I(impl), parent, ref)
+  requires Inv(impl)
+  ensures WFImpl(impl)
+  ensures Inv(impl)
+  ensures F.Next(old(Ik(impl)), old(I(impl)), I(impl))
+  modifies impl.Repr
+  {
+    assert impl.graph.Repr !! impl.invRc.Repr;
+    assert WFImpl(impl);
+
+    var parentEl := impl.graph.Get(parent);
+    assert parentEl.Some?;
+    var newParentEl := parentEl.value.(adjList := (parentEl.value.adjList - {ref}));
+    CountBoundedByMemory(impl.graph);
+    var _ := impl.graph.Insert(parent, newParentEl);
+    impl.Repr := {impl} + impl.graph.Repr + impl.invRc.Repr;
+
+    var refEl := impl.graph.Get(ref);
+    assert refEl.Some?;
+    var newRefEl := refEl.value.(rc := refEl.value.rc - 1);
+    CountBoundedByMemory(impl.graph);
+    var _ := impl.graph.Insert(ref, newRefEl);
+    impl.Repr := {impl} + impl.graph.Repr + impl.invRc.Repr;
+
+    var invRcAopt := impl.invRc.Get(refEl.value.rc);
+    assert invRcAopt.Some?;
+    var invRcA := invRcAopt.value - {ref};
+    CountBoundedByMemory(impl.invRc);
+    var _ := impl.invRc.Insert(refEl.value.rc, invRcA);
+    impl.Repr := {impl} + impl.graph.Repr + impl.invRc.Repr;
+
+    var invRcBopt := impl.invRc.Get(refEl.value.rc - 1);
+    var invRcB := UnwrapOr(invRcBopt, {}) + {ref};
+    CountBoundedByMemory(impl.invRc);
+    var _ := impl.invRc.Insert(refEl.value.rc - 1, invRcB);
+    impl.Repr := {impl} + impl.graph.Repr + impl.invRc.Repr;
+
+    assert I(impl) == F.Detach(old(Ik(impl)), old(I(impl)), parent, ref);
+    F.RefinesDetach(old(Ik(impl)), old(I(impl)), I(impl), parent, ref);
+    assert F.NextStep(old(Ik(impl)), old(I(impl)), I(impl), F.DetachStep(parent, ref));
   }
 }
